## Example 1:

**Theory**

$\vec{F} = m * g$

$g = -9.8\text{ m/s}$ (Of the earth)

$\vec{v_i} = 19.6\text{ m/s}$

$\vec{a_g} = -9.8\frac{m}{s^2}$

$\vec{s} = \vec{v}_{avg}\Delta t \rightarrow \frac{\vec{v}_i + \vec{v}_f}{2} * \Delta t$ (Applies only if acceleration is constant)

$\vec{s} = \frac{\vec{v}_i + \vec{v}_f}{2} * \Delta t \rightarrow \frac{\vec{v}_i + (\vec{v}_i + \vec{a}*\Delta t)}{2} * \Delta t \rightarrow (\frac{2\vec{v}_i}{2} + \frac{\vec{a} * \Delta t}{2}) * \Delta t$ (the $\vec{v}_f = (\vec{v}_i + \vec{a}*\Delta t)$ comes from acceleration being constant)

$\vec{s} = \vec{v}_i * \Delta t + \frac{1}{2} * \vec{a} * (\Delta t)^2$

similarly

$d = v_i t + \frac{1}{2}at^2$

$$
$$
